fin lemme affaiblissement

Meta.v
@@ -8,6 +8,8 @@ Local Open Scope lazy_bool_scope.
 Local Open Scope string_scope.
 Local Open Scope eqb_scope.
 
+Hint Extern 10 => varsdec : sets.
+
 Lemma closed_bsubst n u t :
  term_closed t = true -> term_bsubst n u t = t.
 Proof.
@@ -21,6 +23,7 @@ Proof.
  intros H. f_equal. apply IH. omega with *. apply IH'. omega with *.
 Qed.
 
+(*
 Lemma freevars_fsubst v u t :
  ~Vars.In v (term_fvars t) -> term_fsubst v u t = t.
 Proof.
@@ -33,7 +36,6 @@ Proof.
    intros H. f_equal. apply IH. varsdec. apply IH'. varsdec.
 Qed.
 
-(*
 Lemma term_fsubst_bsubst v t n u T :
   ~Vars.In v (term_fvars u) ->
   term_closed t = true ->
@@ -74,6 +76,13 @@ Definition subvars (sub : subst) :=
 Definition sub_closed (sub : subst) :=
   forallb (fun '(_,t) => term_closed t) sub.
 
+Lemma subinvars_in sub (z:variable) :
+ Vars.In z (subinvars sub) <-> In z (map fst sub).
+Proof.
+ induction sub as [|(a,u) sub IH]; simpl;
+  rewrite <- ?IH; auto with sets.
+Qed.
+
 Lemma list_assoc_suboutvars sub t v :
  list_assoc v sub = Some t ->
  Vars.Subset (term_fvars t) (suboutvars sub).
@@ -85,76 +94,215 @@ Proof.
    + intros NE H. specialize (IH H). varsdec.
 Qed.
 
-Lemma term_fresh_fsubsts sub t :
-  Vars.Subset (term_fvars (term_fsubsts sub t))
-              (Vars.union (term_fvars t) (subvars sub)).
+Lemma term_vmap_ext h h' t :
+ (forall v:variable, Vars.In v (term_fvars t) -> h v = h' v) ->
+ term_vmap h t = term_vmap h' t.
+Proof.
+ revert t.
+ fix IH 1; destruct t; simpl; intros E; trivial.
+ - auto with sets.
+ - f_equal. clear f. revert l E.
+   fix IH' 1; destruct l; simpl; intros; f_equal; auto with sets.
+Qed.
+
+Lemma term_vmap_id h t :
+ (forall v:variable, Vars.In v (term_fvars t) -> h v = FVar v) ->
+ term_vmap h t = t.
+Proof.
+ revert t.
+ fix IH 1; destruct t; simpl; intros E; trivial.
+ - auto with sets.
+ - f_equal. clear f. revert l E.
+   fix IH' 1; destruct l; simpl; intros; f_equal; auto with sets.
+Qed.
+
+Lemma term_vmap_vmap h h' t :
+ term_vmap h (term_vmap h' t) =
+ term_vmap (fun v => term_vmap h (h' v)) t.
+Proof.
+ revert t.
+ fix IH 1; destruct t; simpl; trivial.
+ f_equal. clear f. revert l.
+ fix IH' 1; destruct l; simpl; f_equal; auto.
+Qed.
+
+Lemma form_vmap_ext h h' f :
+ (forall v:variable, Vars.In v (freevars f) -> h v = h' v) ->
+ form_vmap h f = form_vmap h' f.
+Proof.
+ induction f; simpl; intro; f_equal; auto with sets.
+ now injection (term_vmap_ext h h' (Fun "" l)).
+Qed.
+
+Lemma form_vmap_id h f :
+ (forall v:variable, Vars.In v (freevars f) -> h v = FVar v) ->
+ form_vmap h f = f.
+Proof.
+ induction f; simpl; intro; f_equal; auto with sets.
+ now injection (term_vmap_id h (Fun "" l)).
+Qed.
+
+Lemma form_vmap_vmap h h' f :
+ form_vmap h (form_vmap h' f) =
+ form_vmap (fun v => term_vmap h (h' v)) f.
+Proof.
+ induction f; simpl; f_equal; auto.
+ now injection (term_vmap_vmap h h' (Fun "" l)).
+Qed.
+
+Lemma ctx_vmap_ext h h' c :
+ (forall v:variable, Vars.In v (freevars_ctx c) -> h v = h' v) ->
+ ctx_vmap h c = ctx_vmap h' c.
+Proof.
+ induction c; simpl; intros; f_equal;
+  auto using form_vmap_ext with sets.
+Qed.
+
+Lemma ctx_vmap_id h c :
+ (forall v:variable, Vars.In v (freevars_ctx c) -> h v = FVar v) ->
+ ctx_vmap h c = c.
+Proof.
+ induction c; simpl; intros; f_equal;
+  auto using form_vmap_id with sets.
+Qed.
+
+Lemma ctx_vmap_vmap h h' c :
+ ctx_vmap h (ctx_vmap h' c) =
+ ctx_vmap (fun v => term_vmap h (h' v)) c.
+Proof.
+ induction c; simpl; f_equal; auto using form_vmap_vmap with sets.
+Qed.
+
+Lemma ctx_fsubsts_alt sub c :
+ ctx_fsubsts sub c = ctx_vmap (fsubsts sub) c.
+Proof.
+ reflexivity.
+Qed.
+
+(*
+Lemma term_fvars_vmap h t :
+  Vars.Subset
+    (term_fvars (term_vmap h t))
+    (vars_flatmap (fun v => term_fvars (h v))
+                  (Vars.elements (term_fvars t))).
 Proof.
  revert t.
  fix IH 1. destruct t; simpl.
- - destruct (list_assoc v sub) eqn:E; simpl; [ | varsdec].
-   unfold subvars. apply list_assoc_suboutvars in E. varsdec.
+ - varsdec.
+ - varsdec.
+ - clear f. revert l. fix IH' 1. destruct l; simpl.
+   + varsdec.
+   + specialize (IH t). specialize (IH' l). varsdec.
+*)
+
+Lemma term_fvars_fsubsts sub t :
+  Vars.Subset
+    (term_fvars (term_fsubsts sub t))
+    (Vars.union (suboutvars sub)
+                (Vars.diff (term_fvars t) (subinvars sub))).
+Proof.
+ revert t.
+ fix IH 1. destruct t; simpl.
+ - unfold fsubsts. rewrite ?list_assoc_dft_alt.
+   destruct (list_assoc v sub) eqn:E; simpl.
+   + apply list_assoc_suboutvars in E. varsdec.
+   + rewrite list_assoc_notin, <- subinvars_in in E. varsdec.
  - varsdec.
  - clear f. revert l. fix IH' 1. destruct l; simpl.
    + varsdec.
    + specialize (IH t). specialize (IH' l). varsdec.
 Qed.
 
-Lemma fresh_fsubsts sub f :
-  Vars.Subset (freevars (form_fsubsts sub f))
-              (Vars.union (freevars f) (subvars sub)).
+Lemma fvars_fsubsts sub f :
+  Vars.Subset
+    (freevars (form_fsubsts sub f))
+    (Vars.union (suboutvars sub)
+                (Vars.diff (freevars f) (subinvars sub))).
 Proof.
  induction f; simpl; auto; try varsdec.
- apply (term_fresh_fsubsts sub (Fun "" l)).
+ apply (term_fvars_fsubsts sub (Fun "" l)).
 Qed.
 
-Lemma fresh_fsubsts_ctx sub c :
-  Vars.Subset (freevars_ctx (ctx_fsubsts sub c))
-              (Vars.union (freevars_ctx c) (subvars sub)).
+Lemma fvars_fsubsts_ctx sub c :
+  Vars.Subset
+    (freevars_ctx (ctx_fsubsts sub c))
+    (Vars.union (suboutvars sub)
+                (Vars.diff (freevars_ctx c) (subinvars sub))).
 Proof.
  induction c as [|f c IH]; simpl.
  - varsdec.
- - generalize (fresh_fsubsts sub f). varsdec.
+ - generalize (fvars_fsubsts sub f). varsdec.
 Qed.
 
-Lemma fresh_fsubsts_seq sub s :
-  Vars.Subset (freevars_seq (seq_fsubsts sub s))
-              (Vars.union (freevars_seq s) (subvars sub)).
+Lemma fvars_fsubsts_seq sub s :
+  Vars.Subset
+    (freevars_seq (seq_fsubsts sub s))
+    (Vars.union (suboutvars sub)
+                (Vars.diff (freevars_seq s) (subinvars sub))).
 Proof.
  destruct s as (c,f). simpl.
- generalize (fresh_fsubsts_ctx sub c) (fresh_fsubsts sub f).
+ generalize (fvars_fsubsts_ctx sub c) (fvars_fsubsts sub f).
  varsdec.
 Qed.
 
-Lemma term_fsubsts_notIn sub x u t :
+Lemma term_fsubsts_notIn sub (x:variable) u t :
  ~Vars.In x (term_fvars t) ->
  term_fsubsts ((x, u) :: sub) t = term_fsubsts sub t.
 Proof.
- revert t.
- fix IH 1. destruct t; simpl; auto.
- - case eqbspec; auto. varsdec.
- - intros NI. f_equal. clear f.
-   revert l NI.
-   fix IH' 1. destruct l; simpl; auto.
-   intros NI. f_equal. apply IH; varsdec. apply IH'; varsdec.
+ intros NI. apply term_vmap_ext.
+ intros v IN. unfold fsubsts. rewrite !list_assoc_dft_alt.
+ simpl. case eqbspec; auto with sets.
 Qed.
 
-Lemma form_fsubsts_notIn sub x u A :
+Lemma form_fsubsts_notIn sub (x:variable) u A :
  ~Vars.In x (freevars A) ->
  form_fsubsts ((x, u) :: sub) A = form_fsubsts sub A.
 Proof.
- induction A; simpl; intro NI; f_equal; auto.
- - now injection (term_fsubsts_notIn sub x u (Fun "" l)).
- - apply IHA1. varsdec.
- - apply IHA2. varsdec.
+ intros NI. apply form_vmap_ext.
+ intros v IN. unfold fsubsts. rewrite !list_assoc_dft_alt.
+ simpl. case eqbspec; auto with sets.
 Qed.
 
-Lemma ctx_fsubsts_notIn sub x u c:
+Lemma ctx_fsubsts_notIn sub (x:variable) u c:
  ~Vars.In x (freevars_ctx c) ->
  ctx_fsubsts ((x,u)::sub) c = ctx_fsubsts sub c.
 Proof.
- induction c; simpl; intro NI; f_equal; auto.
- apply form_fsubsts_notIn. varsdec.
- apply IHc. varsdec.
+ intros NI. apply ctx_vmap_ext.
+ intros v IN. unfold fsubsts. rewrite !list_assoc_dft_alt.
+ simpl. case eqbspec; auto with sets.
+Qed.
+
+Lemma term_fsubsts_nop sub t :
+ Vars.Empty (Vars.inter (subinvars sub) (term_fvars t)) ->
+ term_fsubsts sub t = t.
+Proof.
+ intros E. apply term_vmap_id.
+ intros v Hv. unfold fsubsts. rewrite list_assoc_dft_alt.
+ assert (H : ~Vars.In v (subinvars sub)) by varsdec.
+ rewrite subinvars_in, <- list_assoc_notin in H.
+ now rewrite H.
+Qed.
+
+Lemma form_fsubsts_nop sub A :
+ Vars.Empty (Vars.inter (subinvars sub) (freevars A)) ->
+ form_fsubsts sub A = A.
+Proof.
+ intros E. apply form_vmap_id.
+ intros v Hv. unfold fsubsts. rewrite list_assoc_dft_alt.
+ assert (H : ~Vars.In v (subinvars sub)) by varsdec.
+ rewrite subinvars_in, <- list_assoc_notin in H.
+ now rewrite H.
+Qed.
+
+Lemma ctx_fsubsts_nop sub c:
+ Vars.Empty (Vars.inter (subinvars sub) (freevars_ctx c)) ->
+ ctx_fsubsts sub c = c.
+Proof.
+ intros E. apply ctx_vmap_id.
+ intros v Hv. unfold fsubsts. rewrite list_assoc_dft_alt.
+ assert (H : ~Vars.In v (subinvars sub)) by varsdec.
+ rewrite subinvars_in, <- list_assoc_notin in H.
+ now rewrite H.
 Qed.
 
 Lemma term_fsubsts_bsubst sub n u t :
@@ -165,7 +313,8 @@ Proof.
  intros CL.
  revert t.
  fix IH 1. destruct t; simpl; auto.
- - destruct (list_assoc v sub) eqn:E; simpl; auto.
+ - unfold fsubsts; rewrite list_assoc_dft_alt.
+   destruct (list_assoc v sub) eqn:E; simpl; auto.
    symmetry. apply closed_bsubst.
    apply list_assoc_in2 in E.
    unfold sub_closed in CL. rewrite forallb_forall in CL.
@@ -194,7 +343,8 @@ Lemma fsubsts_bsubst_adhoc sub x t A :
 Proof.
  intros.
  rewrite fsubsts_bsubst by trivial.
- simpl. case eqbspec; [intros _ |easy].
+ simpl. unfold fsubsts. rewrite list_assoc_dft_alt. simpl.
+ rewrite eqb_refl.
  f_equal.
  now apply form_fsubsts_notIn.
 Qed.
@@ -205,8 +355,7 @@ Lemma Pr_fsubsts logic s :
   Pr logic (seq_fsubsts sub s).
 Proof.
  induction 1; simpl in *; intros; auto.
- - apply R_Ax. unfold ctx_fsubsts.
-   now apply in_map.
+ - apply R_Ax. now apply in_map.
  - apply R_Not_e with (form_fsubsts sub A); auto.
  - apply R_And_e1 with (form_fsubsts sub B); auto.
  - apply R_And_e2 with (form_fsubsts sub A); auto.
@@ -215,8 +364,8 @@ Proof.
  - set (vars := Vars.union (freevars_seq (Γ⊢A)) (subvars sub)).
    set (z := fresh_var vars).
    apply R_All_i with z.
-   + intros H'. apply (fresh_fsubsts_seq sub (Γ⊢A)) in H'.
-     apply (fresh_var_ok vars). exact H'.
+   + intros H'. apply (fvars_fsubsts_seq sub (Γ⊢A)) in H'.
+     apply (fresh_var_ok vars). unfold subvars in vars. varsdec.
    + specialize (IHPr ((x,FVar z)::sub)).
      rewrite ctx_fsubsts_notIn in IHPr by varsdec.
      rewrite <- fsubsts_bsubst_adhoc with (x:=x); auto. varsdec.
@@ -228,8 +377,8 @@ Proof.
  - set (vars := Vars.union (freevars_seq (A::Γ⊢B)) (subvars sub)).
    set (z := fresh_var vars).
    apply R_Ex_e with z (form_fsubsts sub A).
-   + intros H'. apply (fresh_fsubsts_seq sub (A::Γ⊢B) z) in H'.
-     apply (fresh_var_ok vars). exact H'.
+   + intros H'. apply (fvars_fsubsts_seq sub (A::Γ⊢B) z) in H'.
+     apply (fresh_var_ok vars). unfold subvars in vars. varsdec.
    + now apply IHPr1.
    + specialize (IHPr2 ((x,FVar z)::sub)).
      rewrite ctx_fsubsts_notIn in IHPr2 by varsdec.
@@ -239,19 +388,29 @@ Proof.
  - apply R_Absu with l. auto.
 Qed.
 
-Definition Subset {A} (l l': list A) :=
+Definition ListSubset {A} (l l': list A) :=
   forall a, In a l -> In a l'.
 
 Inductive SubsetSeq : sequent -> sequent -> Prop :=
- | SubSeq Γ Γ' A : Subset Γ Γ' -> SubsetSeq (Γ⊢A) (Γ'⊢A).
+ | SubSeq Γ Γ' A : ListSubset Γ Γ' -> SubsetSeq (Γ⊢A) (Γ'⊢A).
 Hint Constructors SubsetSeq.
 
-Lemma Subset_cons {A} (l l': list A) x :
-  Subset l l' -> Subset (x::l) (x::l').
+Lemma ListSubset_cons {A} (l l': list A) x :
+  ListSubset l l' -> ListSubset (x::l) (x::l').
 Proof.
  intros H y [Hy|Hy]; simpl; auto.
 Qed.
-Hint Resolve Subset_cons.
+Hint Resolve ListSubset_cons.
+
+Lemma ListSubset_map {A B} (f:A->B) (l l': list A) :
+  ListSubset l l' -> ListSubset (map f l) (map f l').
+Proof.
+ intros SU b. rewrite !in_map_iff.
+ intros (a & Ha & Ha'). apply SU in Ha'. now exists a.
+Qed.
+
+Ltac varsdec' :=
+ simpl in *; unfold freevars_seq in *; simpl in *; varsdec.
 
 Lemma Pr_weakening logic s s' :
   Pr logic s ->
@@ -265,8 +424,62 @@ Proof.
  - apply R_And_e2 with A; auto.
  - apply R_Or_e with A B; auto.
  - apply R_Imp_e with A; auto.
- - admit. (*now apply R_All_i with x.*)
- - admit. (*now apply R_Ex_i with t.*)
- - admit. (*now apply R_Ex_e with x A.*)
- - admit.
-Admitted.
+ - set (vars := Vars.add x (freevars_seq (Γ' ⊢ A))).
+   set (z := fresh_var vars).
+   assert (Hz : ~Vars.In z vars) by (apply fresh_var_ok).
+   clearbody z; unfold vars in *; clear vars.
+   set (Γ2 := ctx_fsubsts [(x,FVar z)] Γ').
+   assert (~Vars.In x (freevars_ctx Γ2)).
+   { intros IN. apply fvars_fsubsts_ctx in IN. varsdec'. }
+   assert (PR : Pr l (Γ2 ⊢ ∀A)).
+   { apply R_All_i with x.
+     - varsdec'.
+     - apply IHPr. clear IHPr. constructor.
+       rewrite <- (ctx_fsubsts_nop [(x, FVar z)] Γ) by varsdec'.
+       now apply ListSubset_map. }
+   apply Pr_fsubsts with (sub:=[(z,FVar x)]) in PR; auto.
+   simpl in PR.
+   assert (E : ctx_fsubsts [(z, FVar x)] Γ2 = Γ').
+   { unfold Γ2.
+     rewrite !ctx_fsubsts_alt.
+     rewrite ctx_vmap_vmap. apply ctx_vmap_id.
+     intros v IN. unfold fsubsts. simpl.
+     case eqbspec; simpl; case eqbspec; intros; subst; auto.
+     easy.
+     varsdec'. }
+   rewrite E in PR.
+   rewrite form_fsubsts_nop in PR by varsdec'.
+   trivial.
+ - apply R_Ex_i with t; auto.
+ - set (vars := Vars.add x (freevars_seq (A::Γ' ⊢ B))).
+   set (z := fresh_var vars).
+   assert (Hz : ~Vars.In z vars) by (apply fresh_var_ok).
+   clearbody z; unfold vars in *; clear vars.
+   set (Γ2 := ctx_fsubsts [(x,FVar z)] Γ').
+   assert (~Vars.In x (freevars_ctx Γ2)).
+   { intros IN. apply fvars_fsubsts_ctx in IN. varsdec'. }
+   assert (PR : Pr l (Γ2 ⊢ B)).
+   { apply R_Ex_e with x A.
+     - varsdec'.
+     - apply IHPr1. clear IHPr1 IHPr2. constructor.
+       rewrite <- (ctx_fsubsts_nop [(x, FVar z)] Γ) by varsdec'.
+       now apply ListSubset_map.
+     - apply IHPr2. clear IHPr1 IHPr2. constructor.
+       apply ListSubset_cons.
+       rewrite <- (ctx_fsubsts_nop [(x, FVar z)] Γ) by varsdec'.
+       now apply ListSubset_map. }
+   apply Pr_fsubsts with (sub:=[(z,FVar x)]) in PR; auto.
+   simpl in PR.
+   assert (E : ctx_fsubsts [(z, FVar x)] Γ2 = Γ').
+   { unfold Γ2.
+     rewrite !ctx_fsubsts_alt.
+     rewrite ctx_vmap_vmap. apply ctx_vmap_id.
+     intros v IN. unfold fsubsts. simpl.
+     case eqbspec; simpl; case eqbspec; intros; subst; auto.
+     easy.
+     varsdec'. }
+   rewrite E in PR.
+   rewrite form_fsubsts_nop in PR by varsdec'.
+   trivial.
+ - apply R_Absu with l; auto.
+Qed.
